secure_api/box/experimental_box/Box.PKAE.fst
@@ -32,12 +32,12 @@ let pp = PP (AE.get_ae_flagGT ae_params) (fun n -> n / Spec.Salsa20.blocklen < p
 let kp = AE.create_ae_key_package ODH.id AE_Spec.keylen
 
 let ae_package_log_key = i:ODH.id
-let ae_package_log_value (i:ODH.id) = (ap:AE.ae_package #ODH.id #i #AE_Spec.keylen kp ae_params pp)
-let ae_package_log_range (k:ae_package_log_key) = ae_package_log_value k
-let ae_package_log_inv (f:MM.map' (ae_package_log_key) (ae_package_log_range))  = True
+let ae_package_log_value (rgn:erid) (i:ODH.id) = (ap:AE.ae_package #ODH.id #i #AE_Spec.keylen kp ae_params pp{extends (AE.get_ap_rgn ap) rgn})
+let ae_package_log_range (rgn:erid) (k:ae_package_log_key) = ae_package_log_value rgn k
+let ae_package_log_inv (rgn:erid) (f:MM.map' (ae_package_log_key) (ae_package_log_range rgn))  = True
 
-let ae_package_log (rgn:erid) =
-  MM.t rgn (ae_package_log_key) (ae_package_log_range) (ae_package_log_inv)
+let ae_package_log (log_rgn:erid) (ap_rgn:erid) =
+  MM.t log_rgn (ae_package_log_key) (ae_package_log_range ap_rgn) (ae_package_log_inv ap_rgn)
 
 let zero_nonce = Seq.create H.noncelen (UInt8.uint_to_t 0)
 let hsalsa20_hash input = H.hsalsa20 input zero_nonce
@@ -47,26 +47,195 @@ let odh_params = ODH.OP (ODH_Spec.serialized_point_length) (ODH_Spec.scalar_leng
 noeq abstract type pkae_package =
   | PKAE_P :
     op_rgn:erid ->
-    op: ODH.odh_package #AE_Spec.keylen #(AE.key AE_Spec.keylen #ODH.id) kp odh_params ->
-    ap_log_rgn:erid ->
-    ap_log: ae_package_log ap_log_rgn ->
+    op: ODH.odh_package #AE_Spec.keylen #(AE.key AE_Spec.keylen #ODH.id) kp odh_params{extends (ODH.get_op_rgn op) op_rgn} ->
+    ap_log_rgn:erid{disjoint op_rgn ap_log_rgn} ->
+    ap_rgn:erid{disjoint op_rgn ap_rgn /\ disjoint ap_rgn ap_log_rgn /\ disjoint (ODH.get_op_rgn op) ap_rgn} ->
+    ap_log: ae_package_log ap_log_rgn ap_rgn ->
     pkae_package
 
 val create_pkae_package: rgn:erid -> ST pkae_package
   (requires (fun h0 -> True))
   (ensures (fun h0 pkae_p h1 ->
     modifies (Set.singleton rgn) h0 h1
+    /\ extends (ODH.get_op_rgn pkae_p.op) pkae_p.op_rgn
   ))
 let create_pkae_package rgn =
   let pkae_rgn = new_region rgn in
   let odh_rgn = new_region pkae_rgn in
-  let ap_log_rgn = new_region pkae_rgn in
   let op = ODH.create_odh_package kp odh_params odh_rgn in
-  let ap_log = MM.alloc #ap_log_rgn #ae_package_log_key #ae_package_log_range #ae_package_log_inv in
-  PKAE_P odh_rgn op ap_log_rgn ap_log
+  let ap_log_rgn = new_region pkae_rgn in
+  let ap_rgn = new_region pkae_rgn in
+  let ap_log = MM.alloc #ap_log_rgn #ae_package_log_key #(ae_package_log_range ap_rgn) #(ae_package_log_inv ap_rgn) in
+  PKAE_P odh_rgn op ap_log_rgn ap_rgn ap_log
 
+let pkey = ODH.share odh_params
+let skey = ODH.exponent odh_params
+let nonce = AE.nonce ae_params
+let ciphertext = AE.ciphertext ae_params
 let gen = ODH.gen_dh odh_params
 
-val encrypt: #id:eqtype -> #i:id -> #key_length:(n:nat{n<=32}) -> #kp:KEY.key_package #id key_length (key key_length #id) -> #aparams:ae_parameters{key_length = aparams.keylength} -> #pp:plain_package{ valid_ae_plain_package aparams pp} ->  ap:ae_package #id #i #key_length kp aparams pp -> k:key key_length i -> n:nonce aparams.nonce_length -> p:protected_plain pp i -> ST ciphertext
+#set-options "--z3rlimit 300 --max_ifuel 0 --max_fuel 0"
+val get_ap_from_log: pkae_p:pkae_package -> i:ODH.id -> ST (option (ap:ae_package_log_value pkae_p.ap_rgn i))
+  (requires (fun h0 -> True))
+  (ensures (fun h0 ap h1 ->
+    (match sel h0 pkae_p.ap_log i with
+      | Some ap ->
+        contains h1 (AE.get_ap_log ap)
+        /\ MM.defined pkae_p.ap_log i h1
+        /\ MM.contains pkae_p.ap_log i ap h1
+        /\ witnessed (MM.defined pkae_p.ap_log i)
+        /\ witnessed (MM.contains pkae_p.ap_log i ap)
+      | None -> MM.fresh pkae_p.ap_log i h1)
+    /\ h0 == h1
+    /\ ap == MM.sel (sel h1 pkae_p.ap_log) i
+  ))
 
-let encrypt = ODH.odh_package
+let get_ap_from_log pkae_p i =
+  match MM.lookup pkae_p.ap_log i with
+  | Some ap ->
+    AE.recall_log ap;
+    Some ap
+  | None -> None
+
+
+//#set-options "--z3rlimit 300 --max_ifuel 0 --max_fuel 0"
+//val nonce_freshness_framing_lemma: pkae_p:pkae_package -> i:ODH.id -> n:nonce -> h0:mem -> h1:mem -> Lemma
+//  (requires (
+//    //((modifies (Set.singleton (ODH.get_op_rgn pkae_p.op)) h0 h1 /\ (extends (ODH.get_op_rgn pkae_p.op) pkae_p.op_rgn)) \/ h0 == h1)
+//    (modifies (Set.singleton (ODH.get_op_rgn pkae_p.op)) h0 h1 \/ h0 == h1)
+//    /\ extends (ODH.get_op_rgn pkae_p.op) pkae_p.op_rgn
+//    /\ disjoint (ODH.get_op_rgn pkae_p.op) pkae_p.ap_log_rgn
+//    /\ contains h0 pkae_p.ap_log
+//    /\ (match sel h0 pkae_p.ap_log i with
+//      | Some ap -> contains h0 (AE.get_ap_log ap)
+//      | None -> True)
+//  ))
+//  (ensures (
+//    contains h1 pkae_p.ap_log
+//    /\ (match sel h0 pkae_p.ap_log i with
+//      | Some ap_old ->
+//        let ap_new = Some?.v (sel h1 pkae_p.ap_log i) in
+//        AE.get_ap_log ap_old == AE.get_ap_log ap_new
+//        /\ contains h1 (AE.get_ap_log ap_new)
+//      | None -> True)
+//    ///\ (let ap_option_new = sel h1 pkae_p.ap_log i in
+//    //ap_option_new == ap_option_old
+//    ///\ (Some? ap_option_new)
+//    ///\ AE.get_ap_log (Some?.v ap_option_new) == AE.get_ap_log (Some?.v ap_option_old))
+//  ))
+//let nonce_freshness_framing_lemma pkae_p i n h0 h1 = ()
+
+#set-options "--z3rlimit 300 --max_ifuel 0 --max_fuel 0"
+val encrypt: pkae_package:pkae_package -> pk:pkey -> sk:skey{ODH.get_share_raw pk <> ODH.get_share_raw (ODH.get_exp_share sk)} -> n:nonce -> p:protected_plain pp (ODH.create_id pk (ODH.get_exp_share sk)) -> ST ciphertext
+  (requires (fun h0 ->
+    let i = ODH.create_id pk (ODH.get_exp_share sk) in
+    match sel h0 pkae_package.ap_log i with
+    | Some ap ->
+      contains h0 (AE.get_ap_log ap)
+      /\ AE.nonce_is_unique ap n h0
+    | None -> True
+  ))
+  (ensures (fun h0 c h1 ->
+    let i = ODH.create_id pk (ODH.get_exp_share sk) in
+    let both_honest = ODH.exp_hon sk && ODH.sh_hon pk in
+    let kp_log = ODH.get_op_log pkae_package.op in
+    match sel h0 pkae_package.ap_log i with
+    | Some ap ->
+      ((both_honest /\ ODH.get_flag()) ==>
+        (MM.defined kp_log i h0 ==>
+          modifies (Set.singleton (AE.get_ap_rgn ap)) h0 h1)
+        /\ (MM.fresh kp_log i h0 ==>
+          modifies (Set.union (Set.singleton (AE.get_ap_rgn ap)) (Set.singleton (ODH.get_op_rgn pkae_package.op))) h0 h1))
+      /\ ((~both_honest \/ ~(ODH.get_flag())) ==>
+          (modifies (Set.singleton (AE.get_ap_rgn ap)) h0 h1))
+    | None ->
+      MM.defined pkae_package.ap_log i h1
+      /\ (let ap = Some?.v (sel h1 pkae_package.ap_log i) in
+        sel h1 pkae_package.ap_log == MM.upd (sel h0 pkae_package.ap_log) i ap
+        /\ ((both_honest /\ ODH.get_flag()) ==>
+            (MM.defined kp_log i h0 ==>
+              modifies (Set.union (Set.singleton pkae_package.ap_rgn) (Set.union (Set.singleton pkae_package.ap_log_rgn) (Set.singleton (AE.get_ap_rgn ap)))) h0 h1)
+            /\ (MM.fresh kp_log i h0 ==>
+              modifies (Set.union (Set.singleton pkae_package.ap_rgn) (Set.union (Set.singleton pkae_package.ap_log_rgn) (Set.union (Set.singleton (AE.get_ap_rgn ap)) (Set.singleton (ODH.get_op_rgn pkae_package.op))))) h0 h1))
+        /\ ((~both_honest \/ ~(ODH.get_flag())) ==>
+            (modifies (Set.union (Set.singleton pkae_package.ap_rgn) (Set.union (Set.singleton pkae_package.ap_log_rgn) (Set.singleton (AE.get_ap_rgn ap)))) h0 h1)))
+  ))
+
+#set-options "--z3rlimit 500 --max_ifuel 0 --max_fuel 0"
+let encrypt pkae_package pk sk n p =
+  let i = ODH.create_id pk (ODH.get_exp_share sk) in
+  recall pkae_package.ap_log;
+  let k = ODH.dh_op pkae_package.op pk sk in
+  let ap =
+    match get_ap_from_log pkae_package i with
+    | Some ap ->
+      ap
+    | None ->
+      let h0 = get() in
+      let ap = AE.create_ae_package pkae_package.ap_rgn kp ae_params pp in
+      let h1 = get() in
+      MM.extend pkae_package.ap_log i ap;
+      recall pkae_package.ap_log;
+      AE.recall_log ap;
+      //assert(
+        //let both_honest = ODH.exp_hon sk && ODH.sh_hon pk in
+        //(~both_honest \/ ~(ODH.get_flag())) ==>
+          //(modifies (Set.singleton pkae_package.ap_rgn) h0 h1)
+          ////(modifies (Set.singleton (AE.get_ap_rgn ap)) h0 h1)
+          ////(modifies (Set.singleton pkae_package.ap_log_rgn) h0 h1)
+          ////(modifies (Set.union (Set.singleton pkae_package.ap_log_rgn) (Set.singleton (AE.get_ap_rgn ap))) h0 h1)
+          //);
+      ap
+  in
+  AE.encrypt ap k n p
+
+val decrypt: pkae_package:pkae_package -> pk:pkey -> sk:skey{ODH.get_share_raw pk <> ODH.get_share_raw (ODH.get_exp_share sk)} -> n:nonce -> c:ciphertext -> ST (option (p:protected_plain pp (ODH.create_id pk (ODH.get_exp_share sk))))
+  (requires (fun h0 ->
+    let i = ODH.create_id pk (ODH.get_exp_share sk) in
+    match sel h0 pkae_package.ap_log i with
+    | Some ap ->
+      contains h0 (AE.get_ap_log ap)
+    | None -> True
+  ))
+  (ensures (fun h0 c h1 ->
+    let i = ODH.create_id pk (ODH.get_exp_share sk) in
+    let both_honest = ODH.exp_hon sk && ODH.sh_hon pk in
+    let kp_log = ODH.get_op_log pkae_package.op in
+    match sel h0 pkae_package.ap_log i with
+    | Some ap ->
+      ((both_honest /\ ODH.get_flag()) ==>
+        (MM.defined kp_log i h0 ==>
+          h0 == h1)
+        /\ (MM.fresh kp_log i h0 ==>
+          modifies (Set.singleton (ODH.get_op_rgn pkae_package.op)) h0 h1))
+      /\ ((~both_honest \/ ~(ODH.get_flag())) ==>
+          h0 == h1)
+    | None ->
+      MM.defined pkae_package.ap_log i h1
+      /\ (let ap = Some?.v (sel h1 pkae_package.ap_log i) in
+        sel h1 pkae_package.ap_log == MM.upd (sel h0 pkae_package.ap_log) i ap
+        /\ ((both_honest /\ ODH.get_flag()) ==>
+            (MM.defined kp_log i h0 ==>
+              modifies (Set.union (Set.singleton pkae_package.ap_rgn) (Set.singleton pkae_package.ap_log_rgn)) h0 h1)
+            /\ (MM.fresh kp_log i h0 ==>
+              modifies (Set.union (Set.singleton pkae_package.ap_rgn) (Set.union (Set.singleton pkae_package.ap_log_rgn) (Set.singleton (ODH.get_op_rgn pkae_package.op)))) h0 h1))
+        /\ ((~both_honest \/ ~(ODH.get_flag())) ==>
+            (modifies (Set.union (Set.singleton pkae_package.ap_rgn) (Set.singleton pkae_package.ap_log_rgn)) h0 h1)))
+  ))
+
+let decrypt pkae_package pk sk n c =
+  let i = ODH.create_id pk (ODH.get_exp_share sk) in
+  recall pkae_package.ap_log;
+  let k = ODH.dh_op pkae_package.op pk sk in
+  let ap =
+    match get_ap_from_log pkae_package i with
+    | Some ap ->
+      ap
+    | None ->
+      let ap = AE.create_ae_package pkae_package.ap_rgn kp ae_params pp in
+      MM.extend pkae_package.ap_log i ap;
+      recall pkae_package.ap_log;
+      AE.recall_log ap;
+      ap
+  in
+  AE.decrypt ap k n c
